Lagrange done.

src/specs/EvaluateLagrangePolyOutOfDomain.ec
@@ -38,39 +38,14 @@ module EvaluateLagrangePolyOutOfDomain = {
     ret <- (PurePrimops.mulmod ret denominator (W256.of_int Constants.R));
     return ret;
   }
-
-  (* proc low'(polyNum: uint256, at: uint256): uint256 = { *)
-  (* var ret, omegaPower, tmp267, _10, denominator; *)
-  (*   tmp267 <@ Modexp.low(at, (W256.of_int Constants.DOMAIN_SIZE)); *)
-
-  (*   omegaPower <- (W256.of_int 1); *)
-  (*   if ((bool_of_uint256 polyNum)) *)
-  (*   { *)
-  (*     omegaPower <@ Modexp.low((W256.of_int Constants.OMEGA), polyNum); *)
-  (*   } *)
-    
-  (*   ret <- (PurePrimops.addmod tmp267 ((W256.of_int Constants.R) - W256.one) (W256.of_int Constants.R)); *)
-  (*   if ((bool_of_uint256 (PurePrimops.iszero ret))) *)
-  (*   { *)
-  (*     RevertWithMessage.low(W256.of_int 28, W256.of_int STRING); *)
-  (*   } *)
-    
-  (*   ret <- (PurePrimops.mulmod ret omegaPower (W256.of_int Constants.R)); *)
-  (*   _10 <- ((W256.of_int Constants.R) - omegaPower); *)
-  (*   denominator <- (PurePrimops.addmod at _10 (W256.of_int Constants.R)); *)
-  (*   denominator <- (PurePrimops.mulmod denominator (W256.of_int Constants.DOMAIN_SIZE) (W256.of_int Constants.R)); *)
-  (*   denominator <@ Modexp.low(denominator, ((W256.of_int Constants.R) - (W256.of_int 2))); *)
-  (*   ret <- (PurePrimops.mulmod ret denominator (W256.of_int Constants.R)); *)
-  (*   return ret; *)
-  (* } *)
   
   proc mid(polyNum: int, at: int): int option = {
     var r, omegaPolyNum, atDomainSize, zd1, num, den, inv;
 
     omegaPolyNum <@ Modexp.mid(OMEGA,polyNum);
     atDomainSize <@ Modexp.mid(at, DOMAIN_SIZE); 
+
     zd1 <- (atDomainSize - 1) %% R;
-    
     if(zd1 = 0) { (* (at ^ DOMAIN_SIZE) - 1 = 0 *)
       r <- None;
     } else {
@@ -123,41 +98,8 @@ lemma evaluateLagrangePolyOutOfDomain_extracted_equiv_low:
         sp. skip. by progress.
     qed.
 
-lemma modexp_same (m: mem) (v1 v2 p1 p2 r1 r2 : uint256) : 
-    modexp_memory_footprint (modexp_memory_footprint m v1 p1 r1) v2 p2 r2 =
-    modexp_memory_footprint m v2 p2 r2.
-proof. admit. qed.
-
-(* lemma modexp_pspec (m : mem) (base power : uint256) : *)
-(*     phoare [ Modexp.low : *)
-(*       arg = (base, power) /\ *)
-(*       Primops.memory = m /\ *)
-(*       !Primops.reverted *)
-(*       ==> *)
-(*       !Primops.reverted /\ *)
-(*       Primops.memory = modexp_memory_footprint m base power res /\ *)
-(*       res = W256.of_int (((W256.to_uint base) ^ (W256.to_uint power)) %% R) *)
-(*     ] = 1%r. *)
-(* proof. admit. qed. *)
-
-lemma modexp_low_equiv_mid_test (memory: mem) (value256 power256: uint256):
-    equiv [
-      Modexp.low ~ Modexp.mid:
-      arg{1} = (value256, power256) /\
-      arg{2} = (W256.to_uint value256, W256.to_uint power256) /\
-      !Primops.reverted{1} /\
-      Primops.memory{1} = memory    
-      ==>
-      res{2} = W256.to_uint res{1} /\
-      !Primops.reverted{1} /\
-      0 <= res{2} < R /\
-      Primops.memory{1} = (modexp_memory_footprint memory value256 power256 res{1})
-    ].
-proof. admit. qed.
-
-lemma modexp_low_pspec_revert :
-phoare [ Modexp.low : Primops.reverted ==> Primops.reverted ] = 1%r.
-proof. proc; inline*; wp; by progress. qed.
+pred lagrange_memory_footprint (initial final : mem)  =
+   exists (v1 v2 v3: uint256), final = modexp_memory_footprint initial v1 v2 v3.
 
 lemma evaluateLagrangePolyOutOfDomain_low_equiv_mid (memory : mem) (poly256 at256: uint256):
 equiv [
@@ -167,7 +109,9 @@ equiv [
       !Primops.reverted{1} /\
       Primops.memory{1} = memory
       ==>
-      (!Primops.reverted{1} /\ res{2} = Some (to_uint res{1})%W256)
+      (!Primops.reverted{1} /\
+        lagrange_memory_footprint memory Primops.memory{1} /\
+        res{2} = Some (to_uint res{1})%W256)
       \/
       (Primops.reverted{1} /\ res{2} = None)
     ].
@@ -182,11 +126,11 @@ seq 2 1 : (
   (poly256 = W256.zero /\ Primops.memory{1} = memory))
   /\
   omegaPower{1} = W256.of_int omegaPolyNum{2} /\ 0 <= omegaPolyNum{2} < R
-). sp. 
+). sp.
 case (bool_of_uint256 polyNum{1}).
 (* polyNum != 0 *)
 rcondt{1} 1. by progress.
-call (modexp_low_equiv_mid_test memory (W256.of_int OMEGA) poly256).
+call (modexp_low_equiv_mid memory (W256.of_int OMEGA) poly256).
 (* call{1} (modexp_pspec memory (W256.of_int OMEGA) poly256). *)
 skip. progress. by smt. left. by auto.
 rcondf{1} 1. by progress.
@@ -207,10 +151,10 @@ wp.
 exists* omegaPower{1}. elim* => oP.
 pose mem' := (modexp_memory_footprint memory ((of_int OMEGA))%W256 poly256 oP).
 case (poly256 = W256.zero).
-call{1} (modexp_low_equiv_mid_test memory at256 (W256.of_int DOMAIN_SIZE)).
+call{1} (modexp_low_equiv_mid memory at256 (W256.of_int DOMAIN_SIZE)).
 skip. progress. by smt. by smt().
-call{1} (modexp_low_equiv_mid_test mem' at256 (W256.of_int DOMAIN_SIZE)).
-skip. progress. by smt. by smt(). apply modexp_same.
+call{1} (modexp_low_equiv_mid mem' at256 (W256.of_int DOMAIN_SIZE)).
+skip. progress. by smt. by smt(). apply modexp_memory_footprint_same.
 
 seq 1 1: (#pre /\ ret{1} = W256.of_int zd1{2} /\ 0 <= zd1{2} < R).
 wp. skip. progress.
@@ -258,25 +202,24 @@ omegaPower{1} = (of_int omegaPolyNum{2})%W256 /\
 tmp267{1} = (of_int atDomainSize{2})%W256 /\
 0 <= atDomainSize{2} < R /\
 ret{1} = (of_int num{2})%W256 /\
-0 <= num{2} < R /\
-0 <= zd1{2} < R /\
-0 <= den{2} < R /\
+0 <= num{2} < R /\ 0 <= zd1{2} < R /\ 0 <= den{2} < R /\
 Primops.memory{1} = modexp_memory_footprint memory (of_int den{2})%W256 (W256.of_int (R - 2)) denominator{1} /\
 denominator{1} = W256.of_int inv{2} /\ 0 <= inv{2} < R
 ).
 
 exists* tmp267{1}. elim* => tmp. exists* denominator{1}. elim* => d.
 pose mem' := modexp_memory_footprint memory at256 ((of_int DOMAIN_SIZE))%W256 tmp.
-call{1} (modexp_low_equiv_mid_test mem' d ((W256.of_int R) - (W256.of_int 2))).
-skip. progress. rewrite /mem'. by smt. by smt. apply modexp_same.
-wp. skip. progress. rewrite /mulmod. progress. rewrite !W256.of_uintK !R_mod_W256_R.
+call{1} (modexp_low_equiv_mid mem' d ((W256.of_int R) - (W256.of_int 2))).
+skip. progress. rewrite /mem'. by smt. by smt. apply modexp_memory_footprint_same.
+wp. skip. progress. rewrite /lagrange_memory_footprint. by smt().
+rewrite /mulmod. progress. rewrite !W256.of_uintK !R_mod_W256_R.
 have ->: num{2} %% W256.modulus = num{2}. by smt().
 have ->: inv{2} %% W256.modulus = inv{2}. by smt().
 rewrite mod_R_W256_mod_R. by reflexivity.
 qed.
 
 lemma lagrange_pspec_mid (polyNum at: int) :
-    phoare [ EvaluateLagrangePolyOutOfDomain.mid :
+phoare [ EvaluateLagrangePolyOutOfDomain.mid :
       arg = (polyNum, at)
       ==>
       let opR = OMEGA ^ polyNum %% R in
